\section{Transfer Function}%
\label{closedloop}

State space representation of system \\
$
\begin{equations} \label{ssr}
 \dot x_{1} = x_{2} \\
 \dot x_{2} = aF - bx_{3} \\
 \dot x_{3} = x_{4} \\
 \dot x_{4} = - cF + dx_{3}
\end{equations}
$ \\ \\
Applying Laplace transform on the set of equations.
$
\begin{equations} \label{ll}
sX_{1}(s) = X_{2}(s) \\
sX_{2}(s) =aF(s) - bX_{3}(s) \\
sX_{3}(s) = X_{4}(s) \\
sX_{4}(s) = cF(s) + dX_{3}(s) 
\end{equations}
$ \\ \\
Deriving transfer function for $G_{\theta}(s)$ using $F(s)$ as input variable and angle, $X_{3}(s)$ as output variable. \\ 
\[ G_{\theta}(s) = \frac{\theta (s)}{F(s)} \]
$
\begin{equations} \label{dr}
 sX_{3}(s) = X_{4}(s) \\
 sX_{4}(s) = cF(s) + dX_{3}(s) \\
 
 Substituting into
 
s^2 X_{3} = -cF + dX_{3} \\
s^2 X_{3} - dX_{3} = -cF  \\
(s^2-d) X_{3} = -cF  
\end{equations}
$

\[ G_{\theta}(s) = - \frac{c}{s^2 - d} \]

\pagebreak
Deriving transfer function for $G_{x}(s)$ using $F(s)$ as input variable and horisontal position, $X_{1}(s)$ as output variable. 

\[ G_{x}(s) = \frac{X_{1}(s)}{F(s)} \]
$
\begin{equations} \label{dr}
 sX_{1}(s) = X_{2}(s) \\
 sX_{2}(s) =aF(s) - bX_{3}(s) \\
Substituting
s^2 X_{1} = aF - bX_{3}
\begin{equations}
 
\end{equations}
\[ G_{\theta}(s) =  \frac{s^2}{a-b} \]
